specIR/SIRBCE2.v
@@ -1326,8 +1326,12 @@ Section SIM.
   Let md_tgt: Mod.t := (SIR.module sk p_tgt mi ioh).
   Let mp: ModPair.t := (SimSymbId.mk_mp md_src md_tgt).
 
-  Print Universes.
   Set Printing Universes.
+  Print Universes.
+  (* fsim_step *)
+  (* GENMT.fsim_step *)
+  (* SimModSem.fsim_step *)
+  (* SimModSemUnified.fsim_step *)
   Theorem sim_mod: ModPair.sim mp.
   Proof.
     eapply SimSIR.sim_mod with (ord:=gord) (SO:=eq). eauto.
